generational/spec/GC.Gen.CheneyCorrectness.fst
@@ -16,7 +16,6 @@ open GC.Gen.PromoteUpdate
 open GC.Gen.Cheney
 
 module AllocLemmas = GC.Spec.Allocator.Lemmas
-module Part4 = GC.Gen.CheneyPart4
 
 /// ---------------------------------------------------------------------------
 /// Property 1: Object survival
@@ -36,55 +35,6 @@ let cheney_collect_preserves_objects
   reveal_opaque (`%well_formed_heap) well_formed_heap;
   cheney_promote_preserves_wfh_part1 minor major fp roots;
   update_major_pointers_preserves_objects prom.major_final prom.fwd_map
-
-/// ---------------------------------------------------------------------------
-/// Property 2: well_formed_heap_part1
-/// ---------------------------------------------------------------------------
-
-let cheney_collect_preserves_wfh_part1
-  (minor: minor_state) (major: heap) (fp: U64.t) (roots: seq U64.t)
-  : Lemma (requires well_formed_heap major /\
-                    AllocLemmas.fl_valid major fp (heap_size / U64.v mword) /\
-                    AllocLemmas.fl_chain_terminates major fp (heap_size / U64.v mword))
-          (ensures well_formed_heap_part1 (cheney_collect_spec minor major fp roots).mc_major)
-  =
-  cheney_promote_preserves_wfh_part1 minor major fp roots;
-  let prom = cheney_promote minor major fp roots in
-  update_major_pointers_preserves_wfh_part1 prom.major_final prom.fwd_map
-
-/// ---------------------------------------------------------------------------
-/// Property 2b: Part4 preserved
-/// ---------------------------------------------------------------------------
-
-let cheney_collect_preserves_wfh_part4
-  (minor: minor_state) (major: heap) (fp: U64.t) (roots: seq U64.t)
-  : Lemma (requires well_formed_heap major /\
-                    AllocLemmas.fl_valid major fp (heap_size / U64.v mword) /\
-                    AllocLemmas.fl_chain_terminates major fp (heap_size / U64.v mword) /\
-                    Part4.minor_all_no_infix minor)
-          (ensures well_formed_heap_part4 (cheney_collect_spec minor major fp roots).mc_major)
-  =
-  Part4.cheney_promote_preserves_wfh_part4 minor major fp roots;
-  cheney_promote_preserves_wfh_part1 minor major fp roots;
-  let prom = cheney_promote minor major fp roots in
-  update_major_pointers_preserves_wfh_part4 prom.major_final prom.fwd_map
-
-/// ---------------------------------------------------------------------------
-/// Property 2c: Part3 preserved
-/// ---------------------------------------------------------------------------
-
-let cheney_collect_preserves_wfh_part3
-  (minor: minor_state) (major: heap) (fp: U64.t) (roots: seq U64.t)
-  : Lemma (requires well_formed_heap major /\
-                    AllocLemmas.fl_valid major fp (heap_size / U64.v mword) /\
-                    AllocLemmas.fl_chain_terminates major fp (heap_size / U64.v mword) /\
-                    Part4.minor_all_no_infix minor)
-          (ensures well_formed_heap_part3 (cheney_collect_spec minor major fp roots).mc_major)
-  =
-  Part4.cheney_promote_preserves_wfh_part4 minor major fp roots;
-  cheney_promote_preserves_wfh_part1 minor major fp roots;
-  let prom = cheney_promote minor major fp roots in
-  update_major_pointers_preserves_wfh_part3 prom.major_final prom.fwd_map
 
 /// ---------------------------------------------------------------------------
 /// Property 3: Minor reset
@@ -130,7 +80,10 @@ let cheney_gc_correct
                     res.mc_roots == rewrite_roots roots prom.fwd_map))
   =
   cheney_collect_preserves_objects minor major fp roots;
-  cheney_collect_preserves_wfh_part1 minor major fp roots;
+  // Part 1 preservation (inlined from WFH):
+  cheney_promote_preserves_wfh_part1 minor major fp roots;
+  let prom = cheney_promote minor major fp roots in
+  update_major_pointers_preserves_wfh_part1 prom.major_final prom.fwd_map;
   cheney_collect_resets_minor minor major fp roots;
   cheney_collect_rewrites_roots minor major fp roots;
   cheney_collect_preserves_fl_valid minor major fp roots
